\question % Topic 3 - Functions and sketching graphs, Q4.
Let $n$ be a natural number and define a sequence of functions by
\[
    f_0(x) = \frac{x}{x + 1}, \qquad f_{n + 1}(x) = f_0(f_n(x)).
\]
That is, $f_1(x) = f_0(f_0(x))$, $f_2(x) = f_0(f_1(x))$, $f_3(x) = f_0(f_2(x))$, and so on.

\begin{parts}

\part[2]
Find $f_n(x)$ for $n = 1$ and $n = 2$.

\begin{EnvFullwidth}
\begin{solutionorgrid}[2in]
We have
\begin{align*}
    f_1(x) &= f_0(f_0(x)) & f_2(x) &= f_0(f_1(x))\\
    &= \frac{\frac{x}{x + 1}}{\frac{x}{x + 1} + 1} & &= \frac{\frac{x}{2x + 1}}{\frac{x}{2x + 1} + 1} \\
    &= \frac{\frac{x}{\cancel{x + 1}}}{\frac{x + (x + 1)}{\cancel{x + 1}}} & &= \frac{\frac{x}{\cancel{2x + 1}}}{\frac{x + (2x + 1)}{\cancel{2x + 1}}} \\
    &= \frac{x}{2x + 1}, & &= \frac{x}{3x + 1}.
\end{align*}
\end{solutionorgrid}
\end{EnvFullwidth}

\part[5]
Prove by mathematical induction that $\displaystyle{f_n(x) = \frac{x}{(n + 1)x + 1}}$, for all natural numbers $n$.

\begin{EnvFullwidth}
\begin{solutionorgrid}[4.25in]
\begin{proof}
$P(n)$ is: $\displaystyle{f_n(x) = \frac{x}{(n + 1)x + 1}}$, for all $n \in \N$.

\textbf{Basis}: If $n = 0$, then
\[
	f_0(x) = \frac{x}{(0 + 1)x + 1} = \frac{x}{x + 1}.
\]
So, $P(0)$ is true.

\textbf{Inductive step}: If $P(k)$ is true, then $\displaystyle{f_k(x) = \frac{x}{(k + 1)x + 1}}$, for all $k \in \N$. Now,
\begin{align*}
	f_{k + 1} &= f_0(f_k(x)) \\
	&= \frac{\frac{x}{(k + 1)x + 1}}{\frac{x}{(k + 1)x + 1} + 1} && (\textrm{by hypothesis}) \\
	&= \frac{\frac{x}{\cancel{(k + 1)x + 1}}}{\frac{x + ((k + 1)x + 1)}{\cancel{(k + 1)x + 1}}} \\
	&= \frac{x}{((k + 1) + 1)x + 1}.
\end{align*}
Since $P(0)$ is true and $P(k) \implies P(k + 1)$, by the PMI $\displaystyle{f_n(x) = \frac{x}{(n + 1)x + 1}}$ for all $n \in \N$.
\end{proof}
\end{solutionorgrid}
\end{EnvFullwidth}

\end{parts}
