\question[5] % https://math.stackexchange.com/questions/2538331/odd-function-composition.
Prove Theorem~\ref{thm:composition-of-an-odd-function-with-itself} using mathematical induction.

\begin{EnvFullwidth}
\begin{solutionorgrid}[4.5in]
\begin{proof}
$P(n)$ is: if $f$ is an odd function, then $f^n$ is an odd function, for all $n \in \Z^+$.

\textbf{Basis}: If $n = 1$, then $f^1 = f$. So, $P(1)$ is true.

\textbf{Inductive step}: If $P(k)$ is true, then $f^k$ is an odd function for all $k \in \Z^+$. Now,
\begin{align*}
	f^{k + 1}(-x) &= f(f^k(-x)) \\
	&= f(-f^k(x)) && (\textrm{by hypothesis}) \\
	&= -f(f^k(x)) && (f \textrm{ is odd}) \\
	&= -f^{k + 1}(x).
\end{align*}
Since $P(1)$ is true and $P(k) \implies P(k + 1)$, by the PMI $P(n)$ is true for all $n \in \Z^+$.
\end{proof}
\end{solutionorgrid}
\end{EnvFullwidth}
